refactor: Lint

HepLean/FeynmanDiagrams/Wick/Contract.lean
@@ -25,8 +25,8 @@ open PreFeynmanRule
 inductive WickContract : {n : ℕ} → {c : Fin n → 𝓔} → (str : WickString c final) →
     {k : ℕ} → (b1 : Fin k → Fin n) → (b2 : Fin k → Fin n) → Type where
   | string {n : ℕ} {c : Fin n → 𝓔} {str : WickString c final} : WickContract str Fin.elim0 Fin.elim0
-  | contr {n : ℕ} {c : Fin n → 𝓔} {str : WickString c final}  {k : ℕ}
-    {b1 : Fin k → Fin n}  {b2 : Fin k → Fin n}: (i : Fin n) →
+  | contr {n : ℕ} {c : Fin n → 𝓔} {str : WickString c final} {k : ℕ}
+    {b1 : Fin k → Fin n} {b2 : Fin k → Fin n}: (i : Fin n) →
     (j : Fin n) → (h : c j = ξ (c i)) →
     (hilej : i < j) → (hb1 : ∀ r, b1 r < i) → (hb2i : ∀ r, b2 r ≠ i) → (hb2j : ∀ r, b2 r ≠ j) →
     (w : WickContract str b1 b2) →
@@ -35,7 +35,7 @@ inductive WickContract : {n : ℕ} → {c : Fin n → 𝓔} → (str : WickStrin
 namespace WickContract
 
 /-- The number of nodes of a Wick contraction. -/
-def size {n k : ℕ} {c : Fin n → 𝓔} {str : WickString c final}  {b1 b2 : Fin k → Fin n} :
+def size {n k : ℕ} {c : Fin n → 𝓔} {str : WickString c final} {b1 b2 : Fin k → Fin n} :
     WickContract str b1 b2 → ℕ := fun
   | string => 0
   | contr _ _ _ _ _ _ _ w => w.size + 1
@@ -47,6 +47,7 @@ lemma size_eq_k {n k : ℕ} {c : Fin n → 𝓔} {str : WickString c final} {b1 
   | contr _ _ _ _ _ _ _ w => by
     simpa [size] using w.size_eq_k
 
+/-- The map giving the vertices on the left-hand-side of a contraction. -/
 def boundFst {n k : ℕ} {c : Fin n → 𝓔} {str : WickString c final} {b1 b2 : Fin k → Fin n} :
     WickContract str b1 b2 → Fin k → Fin n := fun _ => b1
 
@@ -74,10 +75,10 @@ lemma boundFst_contr_last {n k : ℕ} {c : Fin n → 𝓔} {str : WickString c f
     (contr i j h hilej hb1 hb2i hb2j w).boundFst (Fin.last k) = i := by
   simp only [boundFst, Fin.snoc_last]
 
-lemma boundFst_strictMono {n k : ℕ} {c : Fin n → 𝓔} {str : WickString c final}  {b1 b2 : Fin k → Fin n} :
-    (w : WickContract str b1 b2) → StrictMono w.boundFst := fun
+lemma boundFst_strictMono {n k : ℕ} {c : Fin n → 𝓔} {str : WickString c final}
+    {b1 b2 : Fin k → Fin n} : (w : WickContract str b1 b2) → StrictMono w.boundFst := fun
   | string => fun k => Fin.elim0 k
-  | contr i j _ _ hb1 _ _  w => by
+  | contr i j _ _ hb1 _ _ w => by
     intro r s hrs
     rcases Fin.eq_castSucc_or_eq_last r with hr | hr
     · obtain ⟨r, hr⟩ := hr
@@ -85,11 +86,11 @@ lemma boundFst_strictMono {n k : ℕ} {c : Fin n → 𝓔} {str : WickString c f
       rcases Fin.eq_castSucc_or_eq_last s with hs | hs
       · obtain ⟨s, hs⟩ := hs
         subst hs
-        simp
+        simp only [boundFst_contr_castSucc]
         apply w.boundFst_strictMono _
         simpa using hrs
       · subst hs
-        simp
+        simp only [boundFst_contr_castSucc, boundFst_contr_last]
         exact hb1 r
     · subst hr
       rcases Fin.eq_castSucc_or_eq_last s with hs | hs
@@ -97,12 +98,13 @@ lemma boundFst_strictMono {n k : ℕ} {c : Fin n → 𝓔} {str : WickString c f
         subst hs
         have hsp := s.prop
         rw [Fin.lt_def] at hrs
-        simp at hrs
+        simp only [Fin.val_last, Fin.coe_castSucc] at hrs
         omega
       · subst hs
         simp at hrs
 
-def boundSnd {n k : ℕ} {c : Fin n → 𝓔} {str : WickString c final}  {b1 b2 : Fin k → Fin n} :
+/-- The map giving the vertices on the right-hand-side of a contraction. -/
+def boundSnd {n k : ℕ} {c : Fin n → 𝓔} {str : WickString c final} {b1 b2 : Fin k → Fin n} :
     WickContract str b1 b2 → Fin k → Fin n := fun _ => b2
 
 @[simp]
@@ -129,8 +131,8 @@ lemma boundSnd_contr_last {n k : ℕ} {c : Fin n → 𝓔} {str : WickString c f
     (contr i j h hilej hb1 hb2i hb2j w).boundSnd (Fin.last k) = j := by
   simp only [boundSnd, Fin.snoc_last]
 
-lemma boundSnd_injective {n k : ℕ} {c : Fin n → 𝓔} {str : WickString c final}  {b1 b2 : Fin k → Fin n} :
-    (w : WickContract str b1 b2) → Function.Injective w.boundSnd := fun
+lemma boundSnd_injective {n k : ℕ} {c : Fin n → 𝓔} {str : WickString c final}
+    {b1 b2 : Fin k → Fin n} : (w : WickContract str b1 b2) → Function.Injective w.boundSnd := fun
   | string => by
     intro i j _
     exact Fin.elim0 i
@@ -142,21 +144,22 @@ lemma boundSnd_injective {n k : ℕ} {c : Fin n → 𝓔} {str : WickString c fi
       rcases Fin.eq_castSucc_or_eq_last s with hs | hs
       · obtain ⟨s, hs⟩ := hs
         subst hs
-        simp at hrs
+        simp only [boundSnd_contr_castSucc] at hrs
         simpa using w.boundSnd_injective hrs
       · subst hs
-        simp at hrs
+        simp only [boundSnd_contr_castSucc, boundSnd_contr_last] at hrs
         exact False.elim (h2j r hrs)
     · subst hr
       rcases Fin.eq_castSucc_or_eq_last s with hs | hs
       · obtain ⟨s, hs⟩ := hs
         subst hs
-        simp at hrs
+        simp only [boundSnd_contr_last, boundSnd_contr_castSucc] at hrs
         exact False.elim (h2j s hrs.symm)
       · subst hs
         rfl
 
-lemma color_boundSnd_eq_dual_boundFst {n k : ℕ} {c : Fin n → 𝓔} {str : WickString c final} {b1 b2 : Fin k → Fin n} :
+lemma color_boundSnd_eq_dual_boundFst {n k : ℕ} {c : Fin n → 𝓔} {str : WickString c final}
+    {b1 b2 : Fin k → Fin n} :
     (w : WickContract str b1 b2) → (i : Fin k) → c (w.boundSnd i) = ξ (c (w.boundFst i)) := fun
   | string => fun i => Fin.elim0 i
   | contr i j hij hilej hi _ _ w => fun r => by
@@ -167,8 +170,9 @@ lemma color_boundSnd_eq_dual_boundFst {n k : ℕ} {c : Fin n → 𝓔} {str : Wi
     · subst hr
       simpa using hij
 
-lemma boundFst_lt_boundSnd {n k : ℕ} {c : Fin n → 𝓔} {str : WickString c final}  {b1 b2 : Fin k → Fin n} :
-    (w : WickContract str b1 b2) → (i : Fin k) → w.boundFst i < w.boundSnd i := fun
+lemma boundFst_lt_boundSnd {n k : ℕ} {c : Fin n → 𝓔} {str : WickString c final}
+    {b1 b2 : Fin k → Fin n} : (w : WickContract str b1 b2) → (i : Fin k) →
+    w.boundFst i < w.boundSnd i := fun
   | string => fun i => Fin.elim0 i
   | contr i j hij hilej hi _ _ w => fun r => by
     rcases Fin.eq_castSucc_or_eq_last r with hr | hr
@@ -176,11 +180,11 @@ lemma boundFst_lt_boundSnd {n k : ℕ} {c : Fin n → 𝓔} {str : WickString c 
       subst hr
       simpa using w.boundFst_lt_boundSnd r
     · subst hr
-      simp
+      simp only [boundFst_contr_last, boundSnd_contr_last]
       exact hilej
 
-lemma boundFst_neq_boundSnd {n k : ℕ} {c : Fin n → 𝓔} {str : WickString c final}  {b1 b2 : Fin k → Fin n} :
-    (w : WickContract str b1 b2) → (r1 r2 : Fin k) → b1 r1 ≠ b2 r2 := fun
+lemma boundFst_neq_boundSnd {n k : ℕ} {c : Fin n → 𝓔} {str : WickString c final}
+    {b1 b2 : Fin k → Fin n} : (w : WickContract str b1 b2) → (r1 r2 : Fin k) → b1 r1 ≠ b2 r2 := fun
   | string => fun i => Fin.elim0 i
   | contr i j _ hilej h1 h2i h2j w => fun r s => by
     rcases Fin.eq_castSucc_or_eq_last r with hr | hr
@@ -191,17 +195,19 @@ lemma boundFst_neq_boundSnd {n k : ℕ} {c : Fin n → 𝓔} {str : WickString c
       simpa using w.boundFst_neq_boundSnd r s
     · obtain ⟨r, hr⟩ := hr
       subst hr hs
-      simp
+      simp only [Fin.snoc_castSucc, Fin.snoc_last, ne_eq]
       have hn := h1 r
       omega
     · obtain ⟨s, hs⟩ := hs
       subst hr hs
-      simp
+      simp only [Fin.snoc_last, Fin.snoc_castSucc, ne_eq]
       exact (h2i s).symm
     · subst hr hs
-      simp
+      simp only [Fin.snoc_last, ne_eq]
       omega
 
+/-- Casts a Wick contraction from `WickContract str b1 b2` to `WickContract str b1' b2'` with a
+  proof that `b1 = b1'` and `b2 = b2'`, and that they are defined from the same `k = k'`. -/
 def castMaps {n k k' : ℕ} {c : Fin n → 𝓔}
     {str : WickString c final} {b1 b2 : Fin k → Fin n} {b1' b2' : Fin k' → Fin n}
     (hk : k = k')
@@ -214,16 +220,16 @@ lemma castMaps_rfl {n k : ℕ} {c : Fin n → 𝓔}{str : WickString c final}
     {b1 b2 : Fin k → Fin n} (w : WickContract str b1 b2) :
     castMaps rfl rfl rfl w = w := rfl
 
-lemma mem_snoc' {n k : ℕ} {c : Fin n → 𝓔} {str : WickString c final}  {b1' b2' : Fin k → Fin n} :
+lemma mem_snoc' {n k : ℕ} {c : Fin n → 𝓔} {str : WickString c final} {b1' b2' : Fin k → Fin n} :
     (w : WickContract str b1' b2') →
-    {k' : ℕ} → (hk' : k'.succ = k ) →
+    {k' : ℕ} → (hk' : k'.succ = k) →
     (b1 b2 : Fin k' → Fin n) → (i j : Fin n) → (h : c j = ξ (c i)) →
     (hilej : i < j) → (hb1 : ∀ r, b1 r < i) → (hb2i : ∀ r, b2 r ≠ i) → (hb2j : ∀ r, b2 r ≠ j) →
-    (hb1' : Fin.snoc b1 i  =  b1' ∘ Fin.cast hk') →
-    (hb2' : Fin.snoc b2 j  = b2' ∘ Fin.cast hk') →
-     ∃ (w' : WickContract str b1 b2), w = castMaps hk' hb1' hb2' (contr i j h hilej hb1 hb2i hb2j w')
-     := fun
-  | string => fun hk'  => by
+    (hb1' : Fin.snoc b1 i = b1' ∘ Fin.cast hk') →
+    (hb2' : Fin.snoc b2 j = b2' ∘ Fin.cast hk') →
+    ∃ (w' : WickContract str b1 b2), w = castMaps hk' hb1' hb2' (
+      contr i j h hilej hb1 hb2i hb2j w') := fun
+  | string => fun hk' => by
     simp at hk'
   | contr i' j' h' hilej' hb1' hb2i' hb2j' w' => by
     intro hk b1 b2 i j h hilej hb1 hb2i hb2j hb1' hb2'
@@ -244,31 +250,27 @@ lemma mem_snoc' {n k : ℕ} {c : Fin n → 𝓔} {str : WickString c final}  {b1
       · rw [hb1']
         simp
     have hi : i = i' := by
-      trans  (@Fin.snoc k' (fun _ => Fin n) b1 i) (Fin.last k')
+      trans (@Fin.snoc k' (fun _ => Fin n) b1 i) (Fin.last k')
       · simp
       · rw [hb1']
         simp
     have hj : j = j' := by
-      trans  (@Fin.snoc k' (fun _ => Fin n) b2 j) (Fin.last k')
+      trans (@Fin.snoc k' (fun _ => Fin n) b2 j) (Fin.last k')
       · simp
       · rw [hb2']
         simp
     subst hb1'' hb2'' hi hj
     simp
 
-
-lemma mem_snoc {n k : ℕ} {c : Fin n → 𝓔} {str : WickString c final}  {b1 b2 : Fin k → Fin n} (i j : Fin n)
-    (h : c j = ξ (c i))
-    (hilej : i < j)
-    (hb1 : ∀ r, b1 r < i)
-    (hb2i : ∀ r, b2 r ≠ i)
-    (hb2j : ∀ r, b2 r ≠ j)
+lemma mem_snoc {n k : ℕ} {c : Fin n → 𝓔} {str : WickString c final} {b1 b2 : Fin k → Fin n}
+    (i j : Fin n) (h : c j = ξ (c i)) (hilej : i < j) (hb1 : ∀ r, b1 r < i)
+    (hb2i : ∀ r, b2 r ≠ i) (hb2j : ∀ r, b2 r ≠ j)
     (w : WickContract str (Fin.snoc b1 i) (Fin.snoc b2 j)) :
     ∃ (w' : WickContract str b1 b2), w = contr i j h hilej hb1 hb2i hb2j w' := by
   exact mem_snoc' w rfl b1 b2 i j h hilej hb1 hb2i hb2j rfl rfl
 
-lemma is_subsingleton {n k : ℕ} {c : Fin n → 𝓔} {str : WickString c final}  {b1 b2 : Fin k → Fin n} :
-    Subsingleton (WickContract str b1 b2) := Subsingleton.intro fun w1 w2  => by
+lemma is_subsingleton {n k : ℕ} {c : Fin n → 𝓔} {str : WickString c final} {b1 b2 : Fin k → Fin n} :
+    Subsingleton (WickContract str b1 b2) := Subsingleton.intro fun w1 w2 => by
   induction k with
   | zero =>
     have hb1 : b1 = Fin.elim0 := Subsingleton.elim _ _
@@ -284,7 +286,7 @@ lemma is_subsingleton {n k : ℕ} {c : Fin n → 𝓔} {str : WickString c final
       apply congrArg (contr i j _ _ _ _ _) (hI w w')
 
 lemma eq_snoc_castSucc {k n : ℕ} (b1 : Fin k.succ → Fin n) :
-  b1 = Fin.snoc (b1 ∘ Fin.castSucc) (b1 (Fin.last k)) := by
+    b1 = Fin.snoc (b1 ∘ Fin.castSucc) (b1 (Fin.last k)) := by
   funext i
   rcases Fin.eq_castSucc_or_eq_last i with h1 | h1
   · obtain ⟨i, rfl⟩ := h1
@@ -292,6 +294,9 @@ lemma eq_snoc_castSucc {k n : ℕ} (b1 : Fin k.succ → Fin n) :
   · subst h1
     simp
 
+/-- The construction of a Wick contraction from maps `b1 b2 : Fin k → Fin n`, with the former
+  giving the first index to be contracted, and the latter the second index. These
+  maps must satisfy a series of conditions. -/
 def fromMaps {n k : ℕ} {c : Fin n → 𝓔} {str : WickString c final} (b1 b2 : Fin k → Fin n)
     (hi : ∀ i, c (b2 i) = ξ (c (b1 i)))
     (hb1ltb2 : ∀ i, b1 i < b2 i)
@@ -312,16 +317,18 @@ def fromMaps {n k : ℕ} {c : Fin n → 𝓔} {str : WickString c final} (b1 b2 
         (hb1ltb2 (Fin.last k))
         (fun r => hb1 (Fin.castSucc_lt_last r))
         (fun r a => hb1neb2 (Fin.last k) r.castSucc a.symm)
-        (fun r => hb2.eq_iff.mp.mt (Fin.ne_last_of_lt (Fin.castSucc_lt_last r )))
+        (fun r => hb2.eq_iff.mp.mt (Fin.ne_last_of_lt (Fin.castSucc_lt_last r)))
       (fromMaps (b1 ∘ Fin.castSucc) (b2 ∘ Fin.castSucc) (fun i => hi (Fin.castSucc i))
         (fun i => hb1ltb2 (Fin.castSucc i)) (StrictMono.comp hb1 Fin.strictMono_castSucc)
         ?_ ?_))
     · exact fun r1 r2 => hb1neb2 r1.castSucc r2.castSucc
     · exact Function.Injective.comp hb2 (Fin.castSucc_injective k)
 
-def dropLast {n k : ℕ} {c : Fin n → 𝓔} {str : WickString c final} {b1 b2 : Fin k.succ → Fin n} (w : WickContract str b1 b2) :
-    WickContract str (b1  ∘ Fin.castSucc) (b2 ∘ Fin.castSucc) :=
-  fromMaps (b1  ∘ Fin.castSucc) (b2 ∘ Fin.castSucc)
+/-- Given a Wick contraction with `k.succ` contractions, returns the Wick contraction with
+  `k` contractions by dropping the last contraction (defined by the first index contracted). -/
+def dropLast {n k : ℕ} {c : Fin n → 𝓔} {str : WickString c final} {b1 b2 : Fin k.succ → Fin n}
+    (w : WickContract str b1 b2) : WickContract str (b1 ∘ Fin.castSucc) (b2 ∘ Fin.castSucc) :=
+  fromMaps (b1 ∘ Fin.castSucc) (b2 ∘ Fin.castSucc)
     (fun i => color_boundSnd_eq_dual_boundFst w i.castSucc)
     (fun i => boundFst_lt_boundSnd w i.castSucc)
     (StrictMono.comp w.boundFst_strictMono Fin.strictMono_castSucc)
@@ -331,26 +338,30 @@ def dropLast {n k : ℕ} {c : Fin n → 𝓔} {str : WickString c final} {b1 b2 
 lemma eq_from_maps {n k : ℕ} {c : Fin n → 𝓔} {str : WickString c final} {b1 b2 : Fin k → Fin n}
     (w : WickContract str b1 b2) :
     w = fromMaps w.boundFst w.boundSnd w.color_boundSnd_eq_dual_boundFst
-      w.boundFst_lt_boundSnd w.boundFst_strictMono w.boundFst_neq_boundSnd w.boundSnd_injective := by
-  exact is_subsingleton.allEq w _
+      w.boundFst_lt_boundSnd w.boundFst_strictMono w.boundFst_neq_boundSnd
+      w.boundSnd_injective := is_subsingleton.allEq w _
 
-lemma eq_dropLast_contr {n k : ℕ} {c : Fin n → 𝓔} {str : WickString c final} {b1 b2 : Fin k.succ → Fin n}
-    (w : WickContract str b1 b2) :
+lemma eq_dropLast_contr {n k : ℕ} {c : Fin n → 𝓔} {str : WickString c final}
+    {b1 b2 : Fin k.succ → Fin n} (w : WickContract str b1 b2) :
   w = castMaps rfl (eq_snoc_castSucc b1).symm (eq_snoc_castSucc b2).symm
     (contr (b1 (Fin.last k)) (b2 (Fin.last k))
       (w.color_boundSnd_eq_dual_boundFst (Fin.last k))
       (w.boundFst_lt_boundSnd (Fin.last k))
       (fun r => w.boundFst_strictMono (Fin.castSucc_lt_last r))
       (fun r a => w.boundFst_neq_boundSnd (Fin.last k) r.castSucc a.symm)
-      (fun r => w.boundSnd_injective.eq_iff.mp.mt (Fin.ne_last_of_lt (Fin.castSucc_lt_last r )))
+      (fun r => w.boundSnd_injective.eq_iff.mp.mt (Fin.ne_last_of_lt (Fin.castSucc_lt_last r)))
     (dropLast w)) := by
   rw [eq_from_maps w]
   rfl
 
+/-- Wick contractions of a given Wick string with `k` different contractions. -/
 def Level {n : ℕ} {c : Fin n → 𝓔} (str : WickString c final) (k : ℕ) : Type :=
   Σ (b1 : Fin k → Fin n) (b2 : Fin k → Fin n), WickContract str b1 b2
 
-instance levelZeroFintype {n : ℕ} {c : Fin n → 𝓔} (str : WickString c final) : Fintype (Level str 0) where
+/-- There is a finite number of Wick contractions with no contractions. In particular,
+  this is just the original Wick string.  -/
+instance levelZeroFintype {n : ℕ} {c : Fin n → 𝓔} (str : WickString c final) :
+    Fintype (Level str 0) where
   elems := {⟨Fin.elim0, Fin.elim0, WickContract.string⟩}
   complete := by
     intro x
@@ -362,8 +373,12 @@ instance levelZeroFintype {n : ℕ} {c : Fin n → 𝓔} (str : WickString c fin
       simp only [Finset.mem_singleton]
       rw [is_subsingleton.allEq w string]
 
-structure ContrPair  {n : ℕ} {c : Fin n → 𝓔} {str : WickString c final} {b1 b2 : Fin k → Fin n} (w : WickContract str b1 b2) where
+/-- The pairs of additional indices which can be contracted given a Wick contraction. -/
+structure ContrPair {n : ℕ} {c : Fin n → 𝓔} {str : WickString c final} {b1 b2 : Fin k → Fin n}
+    (w : WickContract str b1 b2) where
+  /-- The first index in the contraction pair. -/
   i : Fin n
+  /-- The second index in the contraction pair. -/
   j : Fin n
   h : c j = ξ (c i)
   hilej : i < j
@@ -371,9 +386,13 @@ structure ContrPair  {n : ℕ} {c : Fin n → 𝓔} {str : WickString c final} {
   hb2i : ∀ r, b2 r ≠ i
   hb2j : ∀ r, b2 r ≠ j
 
-def contrPairEquivSubtype {n : ℕ} {c : Fin n → 𝓔} {str : WickString c final} {b1 b2 : Fin k → Fin n} (w : WickContract str b1 b2) :
+/-- The pairs of additional indices which can be contracted, given an existing wick contraction,
+  is equivalent to the a subtype of `Fin n × Fin n` defined by certain conditions equivalent
+  to the conditions appearing in `ContrPair`. -/
+def contrPairEquivSubtype {n : ℕ} {c : Fin n → 𝓔} {str : WickString c final}
+    {b1 b2 : Fin k → Fin n} (w : WickContract str b1 b2) :
     ContrPair w ≃ {x : Fin n × Fin n // c x.2 = ξ (c x.1) ∧ x.1 < x.2 ∧
-      (∀ r, b1 r < x.1) ∧  (∀ r, b2 r ≠ x.1) ∧ (∀ r, b2 r ≠ x.2)} where
+      (∀ r, b1 r < x.1) ∧ (∀ r, b2 r ≠ x.1) ∧ (∀ r, b2 r ≠ x.2)} where
   toFun cp := ⟨⟨cp.i, cp.j⟩, ⟨cp.h, cp.hilej, cp.hb1, cp.hb2i, cp.hb2j⟩⟩
   invFun x :=
     match x with
@@ -393,16 +412,18 @@ lemma heq_eq {n : ℕ} {c : Fin n → 𝓔} {b1 b2 b1' b2' : Fin k → Fin n} {s
     (w : WickContract str b1 b2)
     (w' : WickContract str b1' b2') (h1 : b1 = b1') (h2 : b2 = b2') : HEq w w':= by
   subst h1 h2
-  simp
+  simp only [heq_eq_eq]
   exact is_subsingleton.allEq w w'
 
+/-- The equivalence between Wick contractions consisting of `k.succ` contractions and
+  those with `k` contractions paired with a suitable contraction pair. -/
 def levelSuccEquiv {n : ℕ} {c : Fin n → 𝓔} (str : WickString c final) (k : ℕ) :
     Level str k.succ ≃ (w : Level str k) × ContrPair w.2.2 where
   toFun w :=
     match w with
     | ⟨b1, b2, w⟩ =>
     ⟨⟨b1 ∘ Fin.castSucc, b2 ∘ Fin.castSucc, dropLast w⟩,
-     ⟨b1 (Fin.last k), b2 (Fin.last k),
+      ⟨b1 (Fin.last k), b2 (Fin.last k),
       w.color_boundSnd_eq_dual_boundFst (Fin.last k),
       w.boundFst_lt_boundSnd (Fin.last k),
       fun r => w.boundFst_strictMono (Fin.castSucc_lt_last r),
@@ -415,7 +436,7 @@ def levelSuccEquiv {n : ℕ} {c : Fin n → 𝓔} (str : WickString c final) (k 
   left_inv w := by
     match w with
     | ⟨b1, b2, w⟩ =>
-      simp
+      simp only [Nat.succ_eq_add_one, Function.comp_apply]
       congr
       · exact Eq.symm (eq_snoc_castSucc b1)
       · funext b2
@@ -429,7 +450,7 @@ def levelSuccEquiv {n : ℕ} {c : Fin n → 𝓔} (str : WickString c final) (k 
   right_inv w := by
     match w with
     | ⟨⟨b1, b2, w⟩, cp⟩ =>
-      simp
+      simp only [Nat.succ_eq_add_one, Fin.snoc_last, Sigma.mk.inj_iff]
       apply And.intro
       · congr
         · exact Fin.snoc_comp_castSucc
@@ -446,38 +467,40 @@ def levelSuccEquiv {n : ℕ} {c : Fin n → 𝓔} (str : WickString c final) (k 
         · simp
         · simp
 
-
-def bound {n k : ℕ} {c : Fin n → 𝓔} {str : WickString c final}  {b1 b2 : Fin k → Fin n}
-    (w : WickContract str b1 b2) : Fin k ⊕ Fin k → Fin n  :=
+/-- The sum of `boundFst` and `boundSnd`, giving on `Sum.inl k` the first index
+  in the `k`th contraction, and on `Sum.inr k` the second index in the `k`th contraction. -/
+def bound {n k : ℕ} {c : Fin n → 𝓔} {str : WickString c final} {b1 b2 : Fin k → Fin n}
+    (w : WickContract str b1 b2) : Fin k ⊕ Fin k → Fin n :=
   Sum.elim w.boundFst w.boundSnd
 
+/-- On `Sum.inl k` the map `bound` acts via `boundFst`. -/
 @[simp]
-lemma bound_inl {n k : ℕ} {c : Fin n → 𝓔} {str : WickString c final}  {b1 b2 : Fin k → Fin n}
+lemma bound_inl {n k : ℕ} {c : Fin n → 𝓔} {str : WickString c final} {b1 b2 : Fin k → Fin n}
     (w : WickContract str b1 b2) (i : Fin k) : w.bound (Sum.inl i) = w.boundFst i := rfl
 
+/-- On `Sum.inr k` the map `bound` acts via `boundSnd`. -/
 @[simp]
-lemma bound_inr {n k : ℕ} {c : Fin n → 𝓔} {str : WickString c final}  {b1 b2 : Fin k → Fin n}
+lemma bound_inr {n k : ℕ} {c : Fin n → 𝓔} {str : WickString c final} {b1 b2 : Fin k → Fin n}
     (w : WickContract str b1 b2) (i : Fin k) : w.bound (Sum.inr i) = w.boundSnd i := rfl
 
-lemma bound_injection {n k : ℕ} {c : Fin n → 𝓔} {str : WickString c final}  {b1 b2 : Fin k → Fin n}
+lemma bound_injection {n k : ℕ} {c : Fin n → 𝓔} {str : WickString c final} {b1 b2 : Fin k → Fin n}
     (w : WickContract str b1 b2) : Function.Injective w.bound := by
   intro x y h
   match x, y with
   | Sum.inl x, Sum.inl y =>
-    simp at h
+    simp only [bound_inl] at h
     simpa using (StrictMono.injective w.boundFst_strictMono).eq_iff.mp h
   | Sum.inr x, Sum.inr y =>
-    simp at h
+    simp only [bound_inr] at h
     simpa using w.boundSnd_injective h
   | Sum.inl x, Sum.inr y =>
-    simp at h
+    simp only [bound_inl, bound_inr] at h
     exact False.elim (w.boundFst_neq_boundSnd x y h)
   | Sum.inr x, Sum.inl y =>
-    simp at h
+    simp only [bound_inr, bound_inl] at h
     exact False.elim (w.boundFst_neq_boundSnd y x h.symm)
 
-
-lemma bound_le_total {n k : ℕ} {c : Fin n → 𝓔} {str : WickString c final}  {b1 b2 : Fin k → Fin n}
+lemma bound_le_total {n k : ℕ} {c : Fin n → 𝓔} {str : WickString c final} {b1 b2 : Fin k → Fin n}
     (w : WickContract str b1 b2) : 2 * k ≤ n := by
   refine Fin.nonempty_embedding_iff.mp ⟨w.bound ∘ finSumFinEquiv.symm ∘ Fin.cast (Nat.two_mul k),
     ?_⟩
@@ -485,39 +508,49 @@ lemma bound_le_total {n k : ℕ} {c : Fin n → 𝓔} {str : WickString c final}
   · exact Fin.cast_injective (Nat.two_mul k)
   · exact bound_injection w
 
+/-- The list of fields (indexed by `Fin n`) in a Wick contraction which are not bound,
+  i.e. which do not appear in any contraction. -/
 def unboundList {n k : ℕ} {c : Fin n → 𝓔} {str : WickString c final} {b1 b2 : Fin k → Fin n}
     (w : WickContract str b1 b2) : List (Fin n) :=
   List.filter (fun i => decide (∀ r, w.bound r ≠ i)) (List.finRange n)
 
 lemma unboundList_nodup {n k : ℕ} {c : Fin n → 𝓔} {str : WickString c final} {b1 b2 : Fin k → Fin n}
-    (w : WickContract str b1 b2) : (w.unboundList).Nodup := List.Nodup.filter _ (List.nodup_finRange n)
+    (w : WickContract str b1 b2) : (w.unboundList).Nodup :=
+    List.Nodup.filter _ (List.nodup_finRange n)
 
-lemma unboundList_length {n k : ℕ} {c : Fin n → 𝓔} {str : WickString c final} {b1 b2 : Fin k → Fin n}
-    (w : WickContract str b1 b2) : w.unboundList.length = n - 2 * k := by
+lemma unboundList_length {n k : ℕ} {c : Fin n → 𝓔} {str : WickString c final}
+    {b1 b2 : Fin k → Fin n} (w : WickContract str b1 b2) :
+    w.unboundList.length = n - 2 * k := by
   rw [← List.Nodup.dedup w.unboundList_nodup]
   rw [← List.card_toFinset, unboundList]
   rw [List.toFinset_filter, List.toFinset_finRange]
-  have hn := Finset.filter_card_add_filter_neg_card_eq_card (s := Finset.univ) (fun (i : Fin n) => i ∈ Finset.image w.bound Finset.univ)
+  have hn := Finset.filter_card_add_filter_neg_card_eq_card (s := Finset.univ)
+    (fun (i : Fin n) => i ∈ Finset.image w.bound Finset.univ)
   have hn' :(Finset.filter (fun i => i ∈ Finset.image w.bound Finset.univ) Finset.univ).card =
       (Finset.image w.bound Finset.univ).card := by
     refine Finset.card_equiv (Equiv.refl _) fun i => ?_
     simp
   rw [hn'] at hn
   rw [Finset.card_image_of_injective] at hn
-  simp only  [Finset.card_univ, Fintype.card_sum, Fintype.card_fin,
+  simp only [Finset.card_univ, Fintype.card_sum, Fintype.card_fin,
     Finset.mem_univ, true_and, Sum.exists, bound_inl, bound_inr, not_or, not_exists] at hn
-  have hn'' : (Finset.filter (fun a => a ∉ Finset.image w.bound Finset.univ) Finset.univ).card = n - 2 * k := by
+  have hn'' : (Finset.filter (fun a => a ∉ Finset.image w.bound Finset.univ) Finset.univ).card =
+      n - 2 * k := by
     omega
   rw [← hn'']
   congr
   funext x
-  simp
+  simp only [ne_eq, Sum.forall, bound_inl, bound_inr, Bool.decide_and, Bool.and_eq_true,
+    decide_eq_true_eq, Finset.mem_image, Finset.mem_univ, true_and, Sum.exists, not_or, not_exists]
   exact bound_injection w
 
-lemma unboundList_sorted {n k : ℕ} {c : Fin n → 𝓔} {str : WickString c final} {b1 b2 : Fin k → Fin n}
-    (w : WickContract str b1 b2) : List.Sorted (fun i j => i < j) w.unboundList :=
+lemma unboundList_sorted {n k : ℕ} {c : Fin n → 𝓔} {str : WickString c final}
+    {b1 b2 : Fin k → Fin n} (w : WickContract str b1 b2) :
+    List.Sorted (fun i j => i < j) w.unboundList :=
   List.Pairwise.sublist (List.filter_sublist (List.finRange n)) (List.pairwise_lt_finRange n)
 
+/-- The map giving the fields which are not bound in a contraction. These
+  are the fields that will appear in a normal operator in Wick's theorem. -/
 def unbound {n k : ℕ} {c : Fin n → 𝓔} {str : WickString c final} {b1 b2 : Fin k → Fin n}
     (w : WickContract str b1 b2) : Fin (n - 2 * k) → Fin n :=
   w.unboundList.get ∘ Fin.cast w.unboundList_length.symm
@@ -529,8 +562,8 @@ lemma unbound_injective {n k : ℕ} {c : Fin n → 𝓔} {str : WickString c fin
     exact w.unboundList_nodup
   · exact Fin.cast_injective _
 
-lemma unbound_strictMono {n k : ℕ} {c : Fin n → 𝓔} {str : WickString c final} {b1 b2 : Fin k → Fin n}
-    (w : WickContract str b1 b2) : StrictMono w.unbound := by
+lemma unbound_strictMono {n k : ℕ} {c : Fin n → 𝓔} {str : WickString c final}
+    {b1 b2 : Fin k → Fin n} (w : WickContract str b1 b2) : StrictMono w.unbound := by
   apply StrictMono.comp
   · refine List.Sorted.get_strictMono w.unboundList_sorted
   · exact fun ⦃a b⦄ a => a
